message invariants for decentralized monotonic

messageInvariantPrototypes/clientServer/decentralizedMonotonic_globalHistory/messageInvariants.dfy
@@ -9,7 +9,7 @@ import opened Obligations
 
 // certified self inductive, modulo requires
 // Every request message in the network has a proper source
-ghost predicate RequestMsgsValidSource(c: Constants, v: Variables) 
+ghost predicate ValidRequestMsgSource(c: Constants, v: Variables) 
   requires v.WF(c)
 {
   forall req | req in v.network.sentMsgs && req.RequestMsg?
@@ -19,57 +19,69 @@ ghost predicate RequestMsgsValidSource(c: Constants, v: Variables)
 // certified self inductive, modulo requires
 // Every request message in the network comes from the source's request set
 // Property of Send
-ghost predicate RequestMsgsValid(c: Constants, v: Variables)
+ghost predicate ValidRequestMessage(c: Constants, v: Variables)
   requires v.WF(c)
-  requires RequestMsgsValidSource(c, v)
+  requires ValidRequestMsgSource(c, v)
 {
-  forall req | req in v.network.sentMsgs && req.RequestMsg?
-  :: req.r.reqId in v.hosts[req.r.clientId].client.requests
+  forall reqMsg | reqMsg in v.network.sentMsgs && reqMsg.RequestMsg?
+  :: 
+    (exists i ::
+      && v.ValidHistoryIdx(i)
+      && reqMsg.r.reqId in v.History(i).hosts[reqMsg.r.clientId].client.requests
+    )
 }
 
-// // certified self inductive, modulo requires
-// // The server's requests must have come from the network
-// // Property of Receive
-// ghost predicate ServerRequestsValid(c: Constants, v: Variables)
-//   requires v.WF(c)
-// {
-//   forall idx:nat, i | c.ValidServerIdx(idx) && 0 <= i < |v.hosts[idx].server.requests|
-//   :: RequestMsg(v.hosts[idx].server.requests[i]) in v.network.sentMsgs
-// }
+// certified self inductive, modulo requires
+// The server's requests must have come from the network
+// Property of Receive
+ghost predicate ServerValidRequest(c: Constants, v: Variables)
+  requires v.WF(c)
+{
+  forall i, idx:nat | 
+    && v.ValidHistoryIdx(i)
+    && c.ValidServerIdx(idx)
+    && v.History(i).hosts[idx].server.currentRequest.Some?
+  :: 
+    RequestMsg(v.History(i).hosts[idx].server.currentRequest.value) in v.network.sentMsgs
+}
 
 
-// // certified self inductive, modulo requires
-// // Every response message in the network comes from the server's requests seq
-// // Property of Send
-// ghost predicate ResponseMsgsValid(c: Constants, v: Variables)
-//   requires v.WF(c)
-// {
-//   forall resp | resp in v.network.sentMsgs && resp.ResponseMsg?
-//   :: (exists i :: 
-//         && 0 <= i < |v.GetServer(c).requests|
-//         && v.GetServer(c).requests[i] == resp.r
-//   )
-// }
+// certified self inductive, modulo requires
+// Every response message in the network comes from the server's request
+// Property of Send
+ghost predicate ValidResponseMessage(c: Constants, v: Variables)
+  requires v.WF(c)
+{
+  forall resp | resp in v.network.sentMsgs && resp.ResponseMsg?
+  :: (exists i :: 
+        && v.ValidHistoryIdx(i)
+        && v.History(i).GetServer(c).server.currentRequest == Some(resp.r)
+  )
+}
 
-// // certified self inductive, modulo requires
-// // Every client's collected responses came from the network.
-// // Property of Receive
-// ghost predicate ClientResponsesValid(c: Constants, v: Variables)
-//   requires v.WF(c)
-// {
-//   forall idx:nat, respId | c.ValidClientIdx(idx) && respId in v.hosts[idx].client.responses
-//   :: ResponseMsg(Req(idx, respId)) in v.network.sentMsgs
-// }
+// certified self inductive, modulo requires
+// Every client's collected responses came from the network.
+// Property of Receive
+ghost predicate ClientResponsesValid(c: Constants, v: Variables)
+  requires v.WF(c)
+{
+  forall i, idx:nat, respId | 
+    && v.ValidHistoryIdx(i)
+    && c.ValidClientIdx(idx) 
+    && respId in v.History(i).hosts[idx].client.responses
+  :: 
+    ResponseMsg(Req(idx, respId)) in v.network.sentMsgs
+}
 
 
 ghost predicate MessageInv(c: Constants, v: Variables) 
 {
   && v.WF(c)
-  // && RequestMsgsValidSource(c, v)
-  // && RequestMsgsValid(c, v)
-  // && ServerRequestsValid(c, v)
-  // && ResponseMsgsValid(c, v)
-  // && ClientResponsesValid(c, v)
+  && ValidRequestMsgSource(c, v)
+  && ValidRequestMessage(c, v)
+  && ServerValidRequest(c, v)
+  && ValidResponseMessage(c, v)
+  && ClientResponsesValid(c, v)
 }
 
 lemma InitImpliesMessageInv(c: Constants, v: Variables)
@@ -82,32 +94,64 @@ lemma MessageInvInductive(c: Constants, v: Variables, v': Variables)
   requires Next(c, v, v')
   ensures MessageInv(c, v')
 {
-  // InvNextResponseMsgsValid(c, v, v');
+  InvNextValidRequestMessage(c, v, v');
+  InvNextServerValidRequest(c, v, v');
+  InvNextValidResponseMessage(c, v, v');
+  InvNextClientResponsesValid(c, v, v');
 }
 
+/***************************************************************************************
+*                                         Proofs                                       *
+***************************************************************************************/
 
-// lemma InvNextResponseMsgsValid(c: Constants, v: Variables, v': Variables)
-//   requires v.WF(c)
-//   requires Next(c, v, v')
-//   requires ResponseMsgsValid(c, v)
-//   ensures ResponseMsgsValid(c, v')
-// {
-//   forall resp | resp in v'.network.sentMsgs && resp.ResponseMsg?
-//   ensures 
-//     exists i :: 
-//       && 0 <= i < |v'.GetServer(c).requests|
-//       && v'.GetServer(c).requests[i] == resp.r
-//   {
-//     var dsStep :| NextStep(c, v, v', dsStep);
-//     var actor, msgOps := dsStep.actorIdx, dsStep.msgOps;
-//     if c.ValidServerIdx(actor) && resp !in v.network.sentMsgs {
-//       var i := |v'.GetServer(c).requests| - 1;  // witness
-//     } else {
-//       // witness and trigger
-//       var i :| 0 <= i < |v.GetServer(c).requests| && v.GetServer(c).requests[i] == resp.r;
-//       assert 0 <= i < |v'.GetServer(c).requests| && v'.GetServer(c).requests[i] == resp.r;
-//     }
-//   }
-// }
+lemma InvNextValidRequestMessage(c: Constants, v: Variables, v': Variables)
+  requires v.WF(c)
+  requires Next(c, v, v')
+  requires ValidRequestMsgSource(c, v)
+  requires ValidRequestMessage(c, v)
+  ensures ValidRequestMessage(c, v')
+{
+  VariableNextProperties(c, v, v');
+}
+
+lemma InvNextServerValidRequest(c: Constants, v: Variables, v': Variables)
+  requires v.WF(c)
+  requires Next(c, v, v')
+  requires ServerValidRequest(c, v)
+  ensures ServerValidRequest(c, v')
+{
+  VariableNextProperties(c, v, v');
+}
+
+lemma InvNextValidResponseMessage(c: Constants, v: Variables, v': Variables)
+  requires v.WF(c)
+  requires Next(c, v, v')
+  requires ValidResponseMessage(c, v)
+  ensures ValidResponseMessage(c, v')
+{
+  VariableNextProperties(c, v, v');
+}
+
+lemma InvNextClientResponsesValid(c: Constants, v: Variables, v': Variables)
+  requires v.WF(c)
+  requires Next(c, v, v')
+  requires ClientResponsesValid(c, v)
+  ensures ClientResponsesValid(c, v')
+{
+  VariableNextProperties(c, v, v');
+}
+
+lemma VariableNextProperties(c: Constants, v: Variables, v': Variables)
+  requires v.WF(c)
+  requires Next(c, v, v')
+  ensures 1 < |v'.history|
+  ensures |v.history| == |v'.history| - 1
+  ensures v.Last() == v.History(|v'.history|-2) == v'.History(|v'.history|-2)
+  ensures forall i | 0 <= i < |v'.history|-1 :: v.History(i) == v'.History(i)
+{
+  assert 0 < |v.history|;
+  assert 1 < |v'.history|;
+}
+
 }  // end module MessageInvariants
 
